## 有理数计算

### 一、口算

(1). $(-16)+(-8)=$	        (2). $-2+12=$		 (3). $-(-2)^3=$

(4). $(-48)÷3=$		         (5). $78+(-85)=$	   (6). $(-14)-(+15)=$

(7). $(-15)+(+9)=$		(8). $(-4)\times (-6)=$	 (9). $4-(-16)=$

(10). $12-(+17)=$		  (11). $84\times(-\frac{1}{3})=$ 	 (12). $\frac{3}{4}÷(-0.25)=$

(13). $4.8-(+2.3)=$		(14). $(-17)-(+9)=$    (15). $0.3\times (-4)=$

(16). $-2^4=$		  	      (17). $(-6)÷(-\frac{1}{3})=$       (18). $\frac{1}{3}-\frac{1}{2}=$

(19). $7.2÷(-2.4)=$	          (20). $\frac{2}{3}\times (-\frac{3}{4})=$           (21). $-7+13=$

(22). $(-1)^{2024}=$ 		       (23). $-10+3.4=$	   (24). $-10-(-3)=$

(25). $\frac{-3^2}{4}=$				(26). $0.42÷(-0.3)=$       (27). $-14÷(-\frac{1}{3})=$

(28). $23-100=$	 	      (29). $-\frac{3}{-4^2}=$



### 二、混合运算 Ⅰ

(1). $\frac{3}{7}÷(-2\frac{1}{7})\times(-64)÷3\frac{1}{5}\times \frac58=$

(2). $-2^2\times (-\frac{1}{2})+8÷(-2)^2=$

(3). $(-39)\frac{17}{18}\times 9=$

(4). $\frac{1}{24}÷(-1+\frac12+\frac13-\frac14)=$

(5). $-4\frac14-(+5\frac13)-(-6\frac12)-(-8\frac13)=$

(6). $-4\frac23\times 0.6+17÷\frac12+(-\frac35)\times(1-\frac13)-17=$

(7). $(-16)+(-5\frac38)+24+(-\frac58)+10=$

(8). $(-2+4)-(-2)\times(-1-3+6)=$



### 三、混合运算 Ⅱ

(1). $(-\frac{1}{2})^{2012}\times(-2)^{2011}=$

(2). $(\frac12-\frac59+\frac56-\frac{7}{12})\times(-36)=$

(3). $-2^3÷(-3)^2\times(-2)=$

(4). $0-2^3÷(-4)^3-\frac18=$

(5). $-5-(-11)+2\frac13-(-\frac23)=$

(6). $-9+5\times(-6)-(-4)^2÷(-8)=$

(7). $100+16÷(-2)^4-\frac15-|-100|=$

(8). $(-1)+(-1)^2+...+(-1)^{2013}=$



### 四、混合运算 Ⅲ

(1). $-4^2÷(-1\frac35)-\frac56\times(-\frac34)=$

(2). $4+(-2)^3\times5-(-0.28)÷4=$

(3). $-36\times(\frac{7}{18}-\frac{3}{4}+\frac{5}{6})-2=$

(4). $7\frac19\times(1\frac12-1\frac18+3\frac14)\times(-2\frac14)=$

(5). $(-3^3+4^2+|-2|)÷3\times(-\frac13)=$

(6). $[4.8\times10^3]÷[(-1\frac35)\times10^2]=$

(7). $-5^2-[(-2)^3+(1-0.8\times\frac34)÷|-1-1|]=$

(8). $(-5)÷[1.85-(2-1\frac34)\times7]=$



### 五、混合运算 Ⅳ

(1). $8\times(-\frac25)-(-4)\times(-\frac29)+(-8)\times\frac35=$

(2). $-6^2÷\frac{2^2}{3}\times(-\frac23)÷(-\frac12)=$

(3). $|-2\frac14|-(-\frac34)+1-|1-\frac12|=$

(4). $(-\frac12)^2+\frac12\times(\frac23-|\frac23-2|)=$

(5). $-1^{2011}-(1-0.5)\times\frac{1}{-2-1}=$

(6). $-\frac{3}{2}\times[-3^2\times(-\frac23)^2-2]=$

(7). $-5^2-[-4+(1-0.2\times\frac15)÷(-2)]=$

(8). $(-81)÷(+2.25)\times\frac49÷16=$

(9). $(-\frac58)\times(-4)^2-0.25\times(-5)\times(-4)^3=$

(10). $(-3)^2-(1\frac12)^3\times\frac29-6÷|-\frac23|=$



### 六、混合运算 Ⅴ

(1). $(-\frac58)\times(-4)^2-0.25\times(-5)\times(-4)^3=$

(2). $(-5)^3\times(-\frac35)^2=$

(3). $|-\frac79|÷(\frac23-\frac15)-\frac13\times(-4)^2=$

(4). $-0.25÷(-\frac12)^2-9\times(-\frac13)^3+(-1)^4÷3=$

(5). $(-5)^3\times(-\frac35)+32÷(-2^2)\times(-1\frac14)=$

(6). $-1^2-[1\frac37+(-12)÷6]^2\times(-\frac34)^2=$

(7). $-4^2÷(-1\frac35)-\frac56\times(-\frac34)=$

(8). $-\frac{3}{-2^3}+\frac{-2}{4^2}-(-\frac12)^3=$

