### 有理数计算

#### 一、口算

$(-16)+(-8)=$

$-2+12=$​

$78+(-85)=$​

$(-14)-(+15)=$​

$(-15)+(+9)=$​

$4-(-16)=$​​

$-10-(-3)=$​

$\frac{1}{3}-\frac{1}{2}=$

$84\times(-\frac{1}{3})=$​

$\frac{3}{4}÷(-0.25)=$​

$\frac{2}{3}\times (-\frac{3}{4})=$​

$7.2÷(-2.4)=$​

$0.42÷(-0.3)=$ 

$-(-2)^3=$

 $(-1)^{2024}=$

$-\frac{3}{-4^2}=$



#### 二、幂运算

$(1÷2)^{-2}-(-5^2)^0+(-\frac14)^{-1}=$







$(4ab^2)^2\times(-\frac12a^2b)^3=$







$已知a^x=2,a^y=3 求a^{x+y}与a^{2x-y}的值$







$3^m=x,3^n=y,用x，y表示3^{3m+2n}$







$若2x+5y-3=0，求4^x\times32^y的值$​







$若(a^nb^mb)^3=a^9b^{15}，求2^{m+n}的值$







#### 三、指数幂化简

$a^2b^3(2a^{-1}b^3)$







$(a^{-2})^{-3}(bc^{-1})^3$







$2(2ab^2c^{-3})^2÷(ab)^{-2}$







#### 五、混合运算

$-2^3÷(-3)^2\times(-2)=$







$-4\frac23\times 0.6+17÷\frac12+(-\frac35)\times(1-\frac13)-17=$







$(-\frac58)\times(-4)^2-0.25\times(-5)\times(-4)^3=$







 $(-\frac{1}{2})^{2012}\times(-2)^{2011}=$







$(-1)+(-1)^2+...+(-1)^{2013}=$

