### 有理数运算

$2 + (-3) = $					$(-5) + (-8) = $			$9 - (-5) = $

$-1.2 + (1\frac15) = $				$-\frac25 - (-\frac35) = $			$1\frac25 - (-2.7) = $

$-25 + 34 + 156 + (-65) = $

$(-3.5) + (-\frac43) + (-\frac34)+(+\frac72) + 0.75 + (-\frac37)= $

$\frac{10}{3} + (-\frac{11}{4}) - (-\frac{5}{6}) + (-\frac{7}{12}) = $

$-9.9 + 10\frac89+9.9+(-10\frac89) = $

$(1\frac34-\frac78-\frac{7}{12})÷(-\frac87) = $

$-12\times(-5)÷[(-3)^2+2\times(-5)] =$

$(-\frac72)\times(\frac16-\frac12)\times\frac{3}{14}÷(-\frac12) =$

$-1^3-(1-\frac12)÷3\times[(-2)^2-5] = $

$\frac23\times(-1.5)+(-\frac23)^2÷\frac49=$

$-3^2+(-24)÷(-4)-(-3)^3\times(-\frac23) = $

$(1-\frac23)÷(-\frac16)+(-3)^2\times(-2) = $

$4÷(\frac23)^2\times(-1)^{2021}-2^2=$

$10-(-9)+(-8)÷2 = $

$18+32÷(-2)^3-(-4)^2\times5 = $

